trying out some things
Signed-off-by: Reto Achermann <reto.achermann@inf.ethz.ch>

CleanQ/CleanQ_SimpleQ.thy
@@ -23,22 +23,55 @@
  *)
 
 theory CleanQ_SimpleQ
-imports "../autocorres/autocorres/AutoCorres"
+  imports 
+    "../autocorres/autocorres/AutoCorres"
+    CleanQ_RB
 begin
 
 external_file "CleanQ_SimpleQ.c"
 
 install_C_file "CleanQ_SimpleQ.c"
-autocorres "CleanQ_SimpleQ.c"
+autocorres [heap_abs_syntax, ts_rules = nondet] "CleanQ_SimpleQ.c"
+
+record foo =   
+  head :: nat
+  tail :: nat
+  size :: nat
 
 context CleanQ_SimpleQ begin
 
 (* Ring Buffer C parser output. *)
 thm rb_init_body_def
+thm rb_init'_def
 thm rb_can_enq_body_def
+thm rb_can_enq'_def
 thm rb_enq_body_def
 thm rb_can_deq_body_def
+
 thm rb_deq_body_def
+
+
+
+
+term rb_C
+
+
+
+
+
+definition rb_C_to_CleanQ_RB :: "lifted_globals \<Rightarrow> rb_C ptr \<Rightarrow> nat  CleanQ_RB"
+  where "rb_C_to_CleanQ_RB s rb = \<lparr>  ring = \<lambda>x. 1,
+                                     head =  Word.unat (head_C (heap_rb_C s rb)), 
+                                     tail =  Word.unat (tail_C (heap_rb_C s rb)),
+                                     size =  Word.unat (size_C (heap_rb_C s rb)) \<rparr>"
+
+lemma foo:
+  "\<lbrace> \<lambda>s.  is_valid_rb_C s rb \<rbrace> rb_can_deq' rb \<lbrace> \<lambda> r s. r = (if rb_can_deq (rb_C_to_CleanQ_RB s rb) then 1 else 0) \<rbrace>!"
+  unfolding  rb_C_to_CleanQ_RB_def rb_can_deq_def rb_empty_def
+  apply(simp)
+  unfolding rb_can_deq'_def
+
+
 
 (* SimpleQ C parser output. *)
 
